FiatFormal/Language/SubstTypeType.v
@@ -4,68 +4,62 @@ Require Import FiatFormal.Language.KiJudge.
 
 (* Substitution of types in types preserves kinding. *)
 Theorem subst_type_type_ix
- :  forall ix ke t1 k1 t2 k2
- ,  get ix ke = Some k2
- -> KIND ke t1 k1
- -> KIND (delete ix ke) t2 k2
- -> KIND (delete ix ke) (substTT ix t2 t1) k1.
+  : forall ix ke t1 k1 t2 k2,
+    get ix ke = Some k2
+    -> KIND ke t1 k1
+    -> KIND (delete ix ke) t2 k2
+    -> KIND (delete ix ke) (substTT ix t2 t1) k1.
 Proof.
  intros. gen ix ke t2 k1 k2.
  induction t1; intros; simpl; inverts H0; eauto.
 
  Case "TVar".
-  destruct k1. destruct k2.
-  fbreak_nat_compare.
-  SCase "n = ix".
-   auto.
+ destruct k1. destruct k2.
+ fbreak_nat_compare.
+ SCase "n = ix".
+ auto.
 
-  SCase "n < ix".
-   apply KIVar. rewrite <- H4.
-   apply get_delete_above; auto.
+ SCase "n < ix".
+ apply KIVar. rewrite <- H4.
+ apply get_delete_above; auto.
 
-  SCase "n > ix".
-   apply KIVar. rewrite <- H4.
-   destruct n.
-    burn.
-    simpl. nnat. apply get_delete_below. omega.
+ SCase "n > ix".
+ apply KIVar. rewrite <- H4.
+ destruct n.
+ burn.
+ simpl. nnat. apply get_delete_below. omega.
 
- (* Case "TForall". *)
- (*  apply KIForall. *)
- (*  rewrite delete_rewind. *)
- (*  eapply IHt1; eauto. *)
- (*  apply liftTT_weaken. auto. *)
+ Case "TExists".
+ apply KIExists.
+ rewrite delete_rewind.
+ eapply IHt1; eauto.
+ apply liftTT_weaken. auto.
 
-  Case "TExists".
-  apply KIExists.
-  rewrite delete_rewind.
-  eapply IHt1; eauto.
-  apply liftTT_weaken. auto.
+ Case "TNProd".
+ apply KINProd.
+ apply Forall_forall; intros.
+ apply map_in_exists in H0. destruct H0 as [y  [YX0  INY]].
+ rewrite Forall_forall in H.
+ specialize (H _ INY).
+ rewrite <- YX0. eapply H.
+ nforall; eauto. eassumption. assumption.
 
-  Case "TNProd".
-  apply KINProd.
-  apply Forall_forall; intros.
-  apply map_in_exists in H0. destruct H0 as [y  [YX0  INY]].
-  rewrite Forall_forall in H.
-  specialize (H _ INY).
-  rewrite <- YX0. eapply H.
-  nforall; eauto. eassumption. assumption.
-
-  Case "TNFun".
-  apply KINFun. eapply IHt1; eassumption.
-  apply Forall_forall; intros.
-  apply map_in_exists in H0. destruct H0 as [y  [YX0  INY]].
-  rewrite Forall_forall in H.
-  specialize (H _ INY).
-  rewrite <- YX0. eapply H; try eassumption.
-  nforall; eauto.
+ Case "TNFun".
+ apply KINFun. eapply IHt1; eassumption.
+ apply Forall_forall; intros.
+ apply map_in_exists in H0. destruct H0 as [y  [YX0  INY]].
+ rewrite Forall_forall in H.
+ specialize (H _ INY).
+ rewrite <- YX0. eapply H; try eassumption.
+ nforall; eauto.
 Qed.
 
 
 Theorem subst_type_type
- :  forall ke t1 k1 t2 k2
- ,  KIND (ke :> k2) t1 k1
- -> KIND ke         t2 k2
- -> KIND ke (substTT 0 t2 t1) k1.
+  : forall ke t1 k1 t2 k2,
+    KIND (ke :> k2) t1 k1
+    -> KIND ke         t2 k2
+    -> KIND ke (substTT 0 t2 t1) k1.
 Proof.
  intros.
  unfold substTT.
